\documentclass[12pt]{article}
\usepackage{fullpage,enumitem,amsmath,amssymb,graphicx}

\begin{document}

\begin{center}
{\Large CSED342 Assignment 8 \vspace{10pt}}

\begin{tabular}{rl}
Student ID: & 20220923 \\
Name: & Yoonhyeok Lee \\
\end{tabular}
\end{center}

\begin{center}
By turning in this assignment, I agree by the POSTECH honor code and declare that all of this is my own work.
\end{center}

\section*{Problem 2a}

This is our given KB.
\begin{align*}
KB = \{(A \lor B ) \rightarrow \lnot C, \lnot (\lnot A \land C) \rightarrow D, A \} \\
\end{align*}
First, we will change each knowledge into CNF.
\begin{align*}
 (A \lor B) \rightarrow \lnot C & \iff \lnot (A \lor B) \lor \lnot C \\
 & \iff (\lnot A \land \lnot B) \lor \lnot C \\
 & \iff (\lnot A \lor \lnot C) \land (\lnot B \lor \lnot C) \\
\lnot (\lnot A \lor C) \rightarrow D & \iff \lnot \lnot (\lnot A \lor C) \lor D  \\
& \iff \lnot A \lor C \lor D  \\
\end{align*}
The resulting KB is this.
\begin{align*}
KB = \{(\lnot A \lor \lnot C) \land (\lnot B \lor \lnot C), \lnot A \lor C \lor D, A\} \\
\end{align*}
Second, split the knowledge and change it into implied form.
\begin{align*}
KB & = \{(\lnot A \lor \lnot C) \land (\lnot B \lor \lnot C), \lnot A \lor C \lor D, A \} \\
& = \{(\lnot A \lor \lnot C) \land (\lnot B \lor \lnot C), (\lnot A \lor C) \lor D, A \} \\
& = \{\lnot A \lor \lnot C, \lnot B \lor \lnot C, \lnot (A \land \lnot C) \lor D, A \} \\
& = \{A \rightarrow \lnot C, B \rightarrow \lnot C, (A, \lnot C) \rightarrow D, A \}  \\
\end{align*}
Third, Use modus ponens.
\begin{align*}
\frac{A \rightarrow \lnot C, A}{\lnot C} , \quad & KB = \{ \lnot C, B \rightarrow \lnot C, (A, \lnot C) \rightarrow D, A\} \\
\frac{(A, \lnot C) \rightarrow D, (A, \lnot C)}{D} , \quad & KB = \{ \lnot C, B \rightarrow \lnot C, D, A\} \\
\end{align*}
Therefore, we can imply D from the given KB.

\section*{Problem 2b}

This is our given KB.
\begin{align*}
KB = \{ A \lor B, B \rightarrow C, (A \lor C) \rightarrow D \}
\end{align*}
First, we will change each knowledge into CNF.
\begin{align*}
B \rightarrow C & \iff \lnot B \lor C \\
(A \lor C) \rightarrow D & \iff \lnot (A \lor C ) \lor D \\
& \iff (\lnot A \land \lnot C) \lor D \\
& \iff (\lnot A \lor D) \land (\lnot C \lor D)
\end{align*}
The resulting KB is this.
\begin{align*}
KB = \{A \lor B, \lnot B \lor C, (\lnot A \lor D) \land (\lnot C \lor D)\}
\end{align*}
Second, split the split the knowledge.
\begin{align*}
KB = \{A \lor B, \lnot B \lor C, \lnot A \lor D, \lnot C \lor D\}
\end{align*}
Third, resolve the knowledge.
\begin{align*}
\frac{A \lor B, \lnot B \lor C}{A \lor C}, & KB = \{A \lor B, \lnot B \lor C, A \lor C, \lnot A \lor D, \lnot C \lor D \} \\
\frac{A \lor C, \lnot A \lor D}{C \lor D}, & KB = \{A \lor B, \lnot B \lor C, A \lor C,C \lor D, \lnot A \lor D, \lnot C \lor D \} \\
\frac{C \lor D, \lnot C \lor D}{D}, & KB = \{A \lor B, \lnot B \lor C, A \lor C,C \lor D, \lnot A \lor D, \lnot C \lor D, D \} \\
\end{align*}
Therefore, we can imply D from the given KB.
\end{document}
